PdlParallelStoring/Examples.lean
@@ -1,35 +1,37 @@
 import PdlParallelStoring.Syntax
 
+open Program
+
 /- Example 1)
    When start to run on input u, stores the initial state u at the second coordinate of an ordered
    pair, then executes actions α and β over the first coordinate of the pair, successively and,
    after that, returns the initial state by restoring the second coordinate. -/
-def π₁ (α β : π) : π :=
-  π.s₂ ;
+def π₁ (α β : Program) : Program :=
+  s₂ ;
   (α ‖ skip) ;
   (β ‖ skip) ;
-  π.r₂
+  r₂
 
 /- Example 2)
    When start to run on input u, stores the initial state u at the second coordinate of an ordered
    pair, then executes action α on the first coordinate of the current pair, until property φ is
    true in the first coordinate of the current pair, then after that, returns to the initial state
    by restoring the second coordinate of the current pair. -/
-def π₂ (α : π) (φ : Φ) : π :=
-  π.s₂ ;
+def π₂ (α : Program) (φ : Formula) : Program :=
+  s₂ ;
   ((((¬ φ) ?) ‖ skip) ; (α ‖ skip))★ ;
   (φ ? ‖ skip) ;
-  π.r₂
+  r₂
 
 /-  Example 3)
     When start to run on input u, stores the initial state u at second coordinate of an ordered
     pair, then executes action α over the first coordinate of the pair and, after that, if property
     φ is true at the initial state then it performs action β over the first coordinate of the
     current pair, else it performs action γ over it. -/
-def π₃ (α β γ : π) (φ : Φ) : π :=
-  π.s₂ ;
+def π₃ (α β γ : Program) (φ : Formula) : Program :=
+  s₂ ;
   (α ‖ skip) ;
-  (((⟨π.r₂ ; φ ?⟩ ⊤') ? ; (β ‖ skip)) ∪ ((⟨π.r₂ ; (¬ φ) ?⟩ ⊤') ? ; (γ ‖ skip)))
+  (((⟨r₂ ; φ ?⟩ ⊤') ? ; (β ‖ skip)) ∪ ((⟨r₂ ; (¬ φ) ?⟩ ⊤') ? ; (γ ‖ skip)))
 
 /-  Example 4)
     When start to run on input u, stores the initial state u at second coordinate of an ordered
@@ -37,7 +39,7 @@ def π₃ (α β γ : π) (φ : Φ) : π :=
     stores the current state as the second coordinate of an ordered pair, executes action α over
     the new first coordinate, and returns to the second pair obtained in the computation; or
     executes action β over the first coordinate of the pair and returns to the initial state. -/
-def π₄ (α β : π) : π :=
-  π.s₂ ;
+def π₄ (α β : Program ) : Program :=
+  s₂ ;
   (α ‖ skip) ;
-  (π.s₂ ; (α ‖ skip) ; π.r₂) ∪ ((β ‖ skip) ; π.r₂)
+  (s₂ ; (α ‖ skip) ; r₂) ∪ ((β ‖ skip) ; r₂)
