PdlParallelStoring/Soundness.lean
@@ -4,7 +4,8 @@ import PdlParallelStoring.Properties
 open Classical
 open Program
 
-lemma soundness_composition (α β : Program) (φ : Formula) : ⊨ ([α ; β] φ) ↔ ([α] [β] φ) := by
+lemma soundness_composition (α β : Program) (φ : Formula) :
+    ⊨ ([α ; β] φ) ↔ ([α] [β] φ) := by
   intros _ _ M _ _ w
   constructor
   . intro hAnd
@@ -29,7 +30,8 @@ lemma soundness_composition (α β : Program) (φ : Formula) : ⊨ ([α ; β] φ
     have hPhiHolds : (M, s) ⊨ φ := hAll t hRwt s hRts
     exact hPhiNotHolds hPhiHolds
 
-lemma soundness_choice (α β : Program) (φ : Formula) : ⊨ ([α ∪ β] φ) ↔ ([α] φ) ∧ ([β] φ) := by
+lemma soundness_choice (α β : Program) (φ : Formula) :
+    ⊨ ([α ∪ β] φ) ↔ ([α] φ) ∧ ([β] φ) := by
   intros _ _ M _ _ w
   constructor
   . intro hAnd
@@ -64,7 +66,8 @@ lemma soundness_choice (α β : Program) (φ : Formula) : ⊨ ([α ∪ β] φ) �
         have hPhiHolds : (M, s) ⊨ φ := hAll₂ s hBeta
         exact hPhiNotHolds hPhiHolds
 
-lemma soundness_k (α : Program) (φ₁ φ₂ : Formula) : ⊨ ([α] φ₁ → φ₂) → ([α] φ₁) → ([α] φ₂) := by
+lemma soundness_k (α : Program) (φ₁ φ₂ : Formula) :
+    ⊨ ([α] φ₁ → φ₂) → ([α] φ₁) → ([α] φ₂) := by
   intros _ _ M _ _ w hAnd
   obtain ⟨hSat₁, hSat₂⟩ := hAnd
   simp only [satisfies, Decidable.not_not, not_exists, not_and] at hSat₁ hSat₂
@@ -76,7 +79,8 @@ lemma soundness_k (α : Program) (φ₁ φ₂ : Formula) : ⊨ ([α] φ₁ → �
   have hPhi₂Holds : (M, s) ⊨ φ₂ := hImp hPhi₁Holds
   exact hPhi₂NotHolds hPhi₂Holds
 
-lemma soundness_functional_r₁ (φ : Formula) : ⊨ (⟨r₁⟩ φ) → ([r₁] φ) := by
+lemma soundness_functional_r₁ (φ : Formula) :
+    ⊨ (⟨r₁⟩ φ) → ([r₁] φ) := by
   intros _ P M _ hEq w hSat
   subst hEq
   simp only [satisfies, Decidable.not_not] at hSat
@@ -93,7 +97,8 @@ lemma soundness_functional_r₁ (φ : Formula) : ⊨ (⟨r₁⟩ φ) → ([r₁]
   rewrite [s'Eq] at hNotSat
   exact hNotSat hSat
 
-lemma soundness_temporal_forward (φ : Formula) : ⊨ φ → ([s₁] ⟨r₁⟩ φ) := by
+lemma soundness_temporal_forward (φ : Formula) :
+    ⊨ φ → ([s₁] ⟨r₁⟩ φ) := by
   intros _ P M _ hEq w hSat
   subst hEq
   simp only [satisfies, Decidable.not_not, not_exists, not_forall, not_and] at hSat
@@ -108,7 +113,8 @@ lemma soundness_temporal_forward (φ : Formula) : ⊨ φ → ([s₁] ⟨r₁⟩ 
   have hNotSat : ¬ (M, w) ⊨ φ := hAll w hR₁
   exact hNotSat hSat₁
 
-lemma soundness_same_domain : ⊨ (⟨r₁⟩ ⊤') ↔ (⟨r₂⟩ ⊤') := by
+lemma soundness_same_domain :
+    ⊨ (⟨r₁⟩ ⊤') ↔ (⟨r₂⟩ ⊤') := by
   intros _ P M _ hEq w
   subst hEq
   constructor
@@ -135,7 +141,8 @@ lemma soundness_same_domain : ⊨ (⟨r₁⟩ ⊤') ↔ (⟨r₂⟩ ⊤') := by
       use s', t
     exact hAll s' hR₁
 
-lemma soundness_unicity (φ : Formula) : ⊨ (⟨s₁ ; r₁⟩ φ) ↔ ([s₁ ; r₁] φ) := by
+lemma soundness_unicity (φ : Formula) :
+    ⊨ (⟨s₁ ; r₁⟩ φ) ↔ ([s₁ ; r₁] φ) := by
   intros _ _ M _ _ w
   constructor
   . intros hAnd
@@ -163,7 +170,8 @@ lemma soundness_unicity (φ : Formula) : ⊨ (⟨s₁ ; r₁⟩ φ) ↔ ([s₁ ;
     have hPhiNotHolds : ¬ (M, w) ⊨ φ := hNeg w hReach
     exact hPhiNotHolds hPhiHolds
 
-lemma soundness_store_restore_id (φ : Formula) : ⊨ ([s₁ ; r₂] φ) → φ := by
+lemma soundness_store_restore_id (φ : Formula) :
+    ⊨ ([s₁ ; r₂] φ) → φ := by
   intros _ _ M _ _ w hAnd
   obtain ⟨hSat, hPhiNotHolds⟩ := hAnd
   simp only
@@ -174,7 +182,8 @@ lemma soundness_store_restore_id (φ : Formula) : ⊨ ([s₁ ; r₂] φ) → φ 
   have hPhiHolds : (M, w) ⊨ φ := hSat w hReach
   exact hPhiNotHolds hPhiHolds
 
-lemma soundness_store_restore_diamond (φ : Formula) : ⊨ φ → ([s₁ ; r₂] ⟨s₁ ; r₂⟩ φ) := by
+lemma soundness_store_restore_diamond (φ : Formula) :
+    ⊨ φ → ([s₁ ; r₂] ⟨s₁ ; r₂⟩ φ) := by
   intros _ _ M _ _ w hAnd
   obtain ⟨hPhiHolds, hSat₂⟩ := hAnd
   simp only [satisfies, Decidable.not_not] at hPhiHolds hSat₂
@@ -199,7 +208,8 @@ lemma soundness_store_restore_iterate (φ : Formula) :
   have hPhiHolds : (M, t) ⊨ φ := hAll t hReach
   exact hPhiNotHolds hPhiHolds
 
-lemma soundness_modus_ponens (φ₁ φ₂ : Formula) (ih₁ : ⊨ φ₁) (ih₂ : ⊨ φ₁ → φ₂) : ⊨ φ₂ := by
+lemma soundness_modus_ponens (φ₁ φ₂ : Formula) (ih₁ : ⊨ φ₁) (ih₂ : ⊨ φ₁ → φ₂) :
+    ⊨ φ₂ := by
   intros _ _ M _ hEq w
   have hSat : (M, w) ⊨ φ₁ := ih₁ hEq
   have hSatInf : (M, w) ⊨ (φ₁ → φ₂) := ih₂ hEq
@@ -211,13 +221,16 @@ lemma soundness_modus_ponens (φ₁ φ₂ : Formula) (ih₁ : ⊨ φ₁) (ih₂ 
     · exact h
   exact hSatInf this
 
-lemma soundness_necessitation (α : Program) (φ : Formula) (ih : ⊨ φ) : ⊨ [α] φ := by
+lemma soundness_necessitation (α : Program) (φ : Formula) (ih : ⊨ φ) :
+    ⊨ [α] φ := by
   intros _ _ M _ hEq w hSat
   obtain ⟨s, _, hPhiNotHolds⟩ := hSat
   have hPhiHolds : (M, s) ⊨ φ := ih hEq
   exact hPhiNotHolds hPhiHolds
 
-theorem soundness_general : ∀ {Γ : Set Formula} {φ : Formula}, (Γ ⊢ φ) → (∀ ψ ∈ Γ, ⊨ ψ) → ⊨ φ := by
+theorem soundness_general :
+    ∀ {Γ : Set Formula} {φ : Formula}, (Γ ⊢ φ) →
+    (∀ ψ ∈ Γ, ⊨ ψ) → ⊨ φ := by
   intros _ _ h
   induction h with
   | premise _ _ hMem =>
@@ -227,9 +240,9 @@ theorem soundness_general : ∀ {Γ : Set Formula} {φ : Formula}, (Γ ⊢ φ) �
   | axiom' _ _ ax =>
       intros
       cases ax with
-      | composition => apply soundness_composition
-      | choice => apply soundness_choice
-      | K => apply soundness_k
+      | modalComposition => apply soundness_composition
+      | modalChoice => apply soundness_choice
+      | modalK => apply soundness_k
       | functionalR₁ => apply soundness_functional_r₁
       | temporalForward => apply soundness_temporal_forward
       | sameDomain => apply soundness_same_domain
@@ -249,7 +262,9 @@ theorem soundness_general : ∀ {Γ : Set Formula} {φ : Formula}, (Γ ⊢ φ) �
       apply ih
       simp only [Set.mem_empty_iff_false, IsEmpty.forall_iff, implies_true]
 
-theorem soundness : ∀ {φ : Formula}, (⊢ φ) → (⊨ φ) := by
+theorem soundness : ∀ {φ : Formula},
+    (⊢ φ) →
+    (⊨ φ) := by
   intros _ h
   apply soundness_general h
   simp only [Set.mem_empty_iff_false, IsEmpty.forall_iff, implies_true]
